Define well-formed kind contexts

src/PlutusIR/Semantics/SemanticEquivalence/FundamentalProperty.v
@@ -13,11 +13,15 @@ Fundamental property (reflexivity) of LR_logically_approximate
 *)
 
 Definition P_has_type Δ Γ e T :=
+  kctx_wf Δ ->
   LR_logically_approximate Δ Γ e e T.
 
-Definition P_constructor_well_formed Δ c Tr := Δ |-ok_c c : Tr.
+Definition P_constructor_well_formed Δ c Tr :=
+  kctx_wf Δ ->
+  Δ |-ok_c c : Tr.
 
 Definition P_bindings_well_formed_nonrec Δ Γ (bs : list binding) :=
+  kctx_wf Δ ->
   forall Δ_t Γ_t bsGn t t' Tn,
     Δ_t = flatten (List.map binds_Delta bs) ++ Δ ->
     map_normalise (flatten (List.map binds_Gamma bs)) bsGn ->
@@ -26,9 +30,12 @@ Definition P_bindings_well_formed_nonrec Δ Γ (bs : list binding) :=
     LR_logically_approximate Δ_t Γ_t t t' Tn ->
     LR_logically_approximate Δ Γ (Let NonRec bs t) (Let NonRec bs t') Tn.
 
-Definition P_bindings_well_formed_rec Δ Γ bs1 := Δ ,, Γ |-oks_r bs1.
+Definition P_bindings_well_formed_rec Δ Γ bs1 :=
+  kctx_wf Δ ->
+  Δ ,, Γ |-oks_r bs1.
 
 Definition P_binding_well_formed Δ Γ b :=
+  kctx_wf Δ ->
   forall Δ_t Γ_t bsGn t t' Tn bs bs',
     Δ_t = binds_Delta b ++ Δ ->
     map_normalise (binds_Gamma b) bsGn ->
@@ -49,8 +56,7 @@ Definition P_binding_well_formed Δ Γ b :=
 
 Lemma LR_reflexivity : forall Δ Γ e T,
     Δ ,, Γ |-+ e : T ->
-    LR_logically_approximate Δ Γ e e T.
-    (* P_has_type Δ Γ e T. *)
+    P_has_type Δ Γ e T.
 Proof with eauto.
   apply has_type__ind with
     (P := P_has_type)
@@ -61,15 +67,15 @@ Proof with eauto.
 
   all : autounfold; intros; subst.
   all : eauto with DSP_compatibility_lemmas typing.
-  - rewrite flatten_app in H5.
-    apply map_normalise__app in H5.
-    destruct H5 as [l1n [l2n [Hmn__l1n [Hmn__l2n Heq]]]].
+  - rewrite flatten_app in H7.
+    apply map_normalise__app in H7.
+    destruct H7 as [l1n [l2n [Hmn__l1n [Hmn__l2n Heq]]]].
     subst.
     eapply map_normalise__deterministic in H1...
     subst.
 
     eapply H0...
-    eapply H3...
+    eapply H4...
     + eapply Kinding.weakening...
       destruct b.
       * simpl. eapply inclusion_refl.
@@ -80,9 +86,9 @@ Proof with eauto.
         -- eapply eqb_eq in Heqb as Heq.
            subst.
            assert (appears_bound_in_ann x (Let NonRec (TypeBind (TyVarDecl x k) t1 :: bs) t)) by eauto.
-           eapply uniqueness' in H4.
-           rewrite H4 in H1.
-           inversion H4.
+           eapply uniqueness' in H6.
+           rewrite H6 in H1.
+           inversion H6.
         -- apply eqb_neq in Heqb as Hneq.
            simpl. rewrite Heqb...
       * destruct d.
@@ -94,9 +100,9 @@ Proof with eauto.
         -- eapply eqb_eq in Heqb as Heq.
            subst.
            assert (appears_bound_in_ann x (Let NonRec (DatatypeBind (Datatype (TyVarDecl x k) l b l0) :: bs) t)) by eauto.
-           eapply uniqueness' in H4.
-           rewrite H4 in H1.
-           inversion H4.
+           eapply uniqueness' in H6.
+           rewrite H6 in H1.
+           inversion H6.
         -- apply eqb_neq in Heqb as Hneq.
            simpl. rewrite Heqb...
     + rewrite app_assoc...
@@ -129,10 +135,16 @@ Hint Unfold P_has_type : hintdb_compat_context.
 
 Lemma LR_reflexivity_context : forall C Δ₁ Γ₁ Δ Γ T T₁,
   Δ₁ ,, Γ₁ |-C C : (Δ ,, Γ ▷ T) ↝ T₁ ->
+  kctx_wf Δ₁ ->
+  kctx_wf Δ ->
   LR_logically_approximate_context Δ₁ Γ₁ C C Δ Γ T T₁.
 Proof with eauto with hintdb_compat_context.
   induction C.
 
-  all: intros Δ₁ Γ₁ Δ Γ T T₁ H_C_ty.
+  all: intros Δ₁ Γ₁ Δ Γ T T₁ H_C_ty H_kctx H_kctx'.
   all: inversion H_C_ty; subst...
+  - eapply compatibility_C_Apply_L...
+    eapply LR_reflexivity...
+  - eapply compatibility_C_Apply_R...
+    eapply LR_reflexivity...
 Qed.
